Removed old yield files:

examples/Yield/Lang.v
@@ -29,13 +29,18 @@ From Coinduction Require Import
 
 From CTree Require Import
      CTree
-     Eq.
+     Eq
+     Eq.WBisim.
 
 From CTreeYield Require Import
      Par.
 
+From Equations Require Import Equations.
+
 Import ListNotations.
-Import MonadNotation.
+(* Import MonadNotation. *)
+Import CTreeNotations.
+Import WBisimNotations.
 Local Open Scope monad_scope.
 Local Open Scope string_scope.
 
@@ -57,8 +62,9 @@ Inductive stmt : Type :=
 | Seq    (a b : stmt)            (* a ; b *)
 | If     (i : expr) (t e : stmt) (* if (i) then { t } else { e } *)
 | While  (t : expr) (b : stmt)   (* while (t) { b } *)
-| Spawn  (t : stmt)              (* spawn t *)
+| Spawn  (t1 t2 : stmt)          (* spawn t1; continue t2 *)
 | Skip                           (* ; *)
+| YieldS                         (* yield *)
 .
 
 Variant ImpState : Type -> Type :=
@@ -66,58 +72,52 @@ Variant ImpState : Type -> Type :=
 | SetVar (x : var) (v : value) : ImpState unit.
 
 Section Denote1.
-  Fixpoint denote_expr (e : expr) : ctree (stateE value +' spawnE) value :=
-    match e with
-    | Var v     => trigger (Get _)
-    | Lit n     => ret n
-    | Plus a b  => l <- denote_expr a ;; r <- denote_expr b ;; ret (l + r)
-    | Minus a b => l <- denote_expr a ;; r <- denote_expr b ;; ret (l - r)
-    | Mult a b  => l <- denote_expr a ;; r <- denote_expr b ;; ret (l * r)
-    end.
-
-  Definition while (step : ctree (stateE value +' spawnE) (unit + unit)) : ctree (stateE value +' spawnE) unit :=
-    CTree.iter (fun _ => step) tt.
-
   Definition is_true (v : value) : bool := if (v =? 0)%nat then false else true.
 
-  Fixpoint denote_imp (s : stmt) : ctree (stateE value +' spawnE) unit :=
-    match s with
-    | Assign x e =>  v <- denote_expr e ;; trigger (Put _ v)
-    | Seq a b    =>  denote_imp a ;; denote_imp b
-    | If i t e   =>
-      v <- denote_expr i ;;
-      if is_true v then denote_imp t else denote_imp e
-
-    | While t b =>
-      while (v <- denote_expr t ;;
-	         if is_true v
-             then denote_imp b ;; ret (inl tt)
-             else ret (inr tt))
-
-    | Spawn t =>
-        b <- trigger Par.Spawn;;
-        match b with
-        | true => denote_imp t;; ChoiceI 0 (fun _ => ret tt) (* force the thread to halt here *)
-        | false => ret tt
-        end
-    | Skip => ret tt
-
-    (* | Atomic t => translate ... (denote_imp t) *)
+  Definition while' (step : ctree (parE value) (unit + unit)) : ctree (parE value) unit :=
+    CTree.iter (fun _ => step) tt.
+  Fixpoint denote_expr' (e : expr) : ctree (parE value) value :=
+    match e with
+    | Var v     => x <- trigger (Get _) ;; trigger Yield;; ret x
+    | Lit n     => ret n
+    | Plus a b  => l <- denote_expr' a ;; r <- denote_expr' b ;; ret (l + r)%nat
+    | Minus a b => l <- denote_expr' a ;; r <- denote_expr' b ;; ret (l - r)
+    | Mult a b  => l <- denote_expr' a ;; r <- denote_expr' b ;; ret (l * r)
     end.
 
-  Definition h_state {E} `{yieldE value -< E} : forall X, stateE value X -> Monads.stateT value (ctree E) X :=
-    fun _ e s =>
-      match e with
-      | Get _ => Ret (s, s)
-      | Put _ s' => Ret (s', tt)
-      end.
+  Fixpoint denote_imp' (s : stmt) : ctree (parE value) unit :=
+    match s with
+    | Assign x e =>  v <- denote_expr' e ;; x <- trigger (Put _ v) ;; ret x
+    | Seq a b    =>  denote_imp' a ;; denote_imp' b
+    | If i t e   =>
+      v <- denote_expr' i ;;
+      if is_true v then denote_imp' t else denote_imp' e
 
-  (* The effects take place, then yields *)
-  Definition h_state_yield {E} `{yieldE value -< E} : forall X, stateE value X -> Monads.stateT value (ctree E) X :=
-    fun _ e s =>
+    | While t b =>
+      while' (v <- denote_expr' t ;;
+	         if is_true v
+             then denote_imp' b ;; ret (inl tt)
+             else ret (inr tt))
+
+    | Spawn t1 t2 =>
+        b <- trigger Par.Spawn;;
+        match b with
+        | true => denote_imp' t1
+        | false => denote_imp' t2
+        end
+    | Skip => ret tt
+    | YieldS => trigger Yield
+    end.
+
+  Definition schedule_denot' (t : stmt) : completed :=
+    schedule 1 (fun _ => denote_imp' t) (Some Fin.F1).
+
+  (*
+  Definition h_state : forall X, stateE value X -> ctree (parE value) X :=
+    fun _ e =>
       match e with
-      | Get _ => s' <- trigger (Yield _ s);; Ret (s', s)
-      | Put _ s' => s'' <- trigger (Yield _ s');; Ret (s'', tt)
+      | Get _ => x <- trigger (Get _) ;; trigger Yield ;; Ret x
+      | Put _ s' => x <- trigger (Put _ s') ;; trigger Yield ;; Ret x
       end.
 
   #[global] Instance MonadChoice_stateT {M S} {MM : Monad M} {AM : Utils.MonadChoice M}
@@ -126,27 +126,26 @@ Section Denote1.
       f <- choice b n;;
       ret (s, f).
 
-  Definition handler : forall X, (stateE value +' spawnE) X -> Monads.stateT value (ctree (parE value)) X :=
-    (fun X (e : (stateE value +' spawnE) X) =>
+  Definition handler : forall X, (spawnE +' stateE value) X -> ctree (parE value) X :=
+    (fun X (e : (spawnE +' stateE value) X) =>
        match e with
-       | inl1 e' => h_state_yield _ e'
-       | inr1 e' =>
-         match e' in spawnE R return Monads.stateT value (ctree (parE value)) R with
-         | Par.Spawn => fun s => b <- trigger Par.Spawn;; Ret(s, b) (* TODO: use MonadTrigger *)
-         end
+       | inl1 e' => trigger e'
+       | inr1 e' => h_state _ e'
        end).
 
-  Definition interp_state (t : ctree (stateE value +' spawnE) unit) : thread :=
+  Definition interp_state (t : ctree (spawnE +' stateE value) unit) : thread :=
     Interp.interp handler t.
 
   Definition schedule_denot (t : stmt) : thread :=
-    schedule' 1 (fun _ => (interp_state (denote_imp t))) Fin.F1.
-
+    schedule 1 (fun _ => interp_state (denote_imp t)) (Some Fin.F1).
+   *)
   Lemma denote_expr_bounded e :
-    choiceI_bound 1 (denote_expr e).
+    choiceI_bound 1 (denote_expr' e).
   Proof.
     induction e; cbn; unfold trigger; auto.
-    - step. constructor. intros. step. constructor.
+    - step. rewrite bind_vis. constructor. intros.
+      step. rewrite bind_ret_l. rewrite bind_vis. constructor. intros.
+      step. rewrite bind_ret_l. constructor.
     - step. constructor.
     - apply bind_choiceI_bound; auto.
       intros. apply bind_choiceI_bound; auto.
@@ -160,15 +159,17 @@ Section Denote1.
   Qed.
 
   Lemma denote_stmt_bounded t :
-    choiceI_bound 1 (denote_imp t).
+    choiceI_bound 1 (denote_imp' t).
   Proof.
     induction t; cbn.
-    - apply bind_choiceI_bound. apply denote_expr_bounded.
-      intros. step. constructor. intros. step. constructor.
+    - apply bind_choiceI_bound. apply denote_expr_bounded. intros.
+      step. rewrite bind_trigger. constructor. intros.
+      (* step. rewrite bind_trigger. constructor. intros. *)
+      step. constructor.
     - apply bind_choiceI_bound; auto.
     - apply bind_choiceI_bound. apply denote_expr_bounded.
       intros. step. step in IHt1. step in IHt2. destruct (is_true x); auto.
-    - unfold while. apply iter_choiceI_bound; auto.
+    - unfold while'. apply iter_choiceI_bound; auto.
       intros. apply bind_choiceI_bound. apply denote_expr_bounded.
       intros. destruct (is_true x).
       + apply bind_choiceI_bound; auto.
@@ -176,67 +177,226 @@ Section Denote1.
       + step. constructor.
     - apply bind_choiceI_bound.
       + intros. step. constructor. intros. step. constructor.
-      + intros. destruct x.
-        * apply bind_choiceI_bound; auto.
-          intros. step. constructor; auto. intros. step. constructor.
-        * step. constructor.
+      + intros. destruct x; auto.
     - step. constructor.
+    - step. constructor. intros. step. constructor.
   Qed.
 
-  (* not used *)
-  Lemma handler_bounded X (e : (stateE value +' spawnE) X) c :
-    choiceI_bound 1 (handler _ e c).
-  Proof.
-    destruct e; destruct s; cbn.
-    - apply bind_choiceI_bound; auto.
-      + step. constructor. intros. step. constructor.
-      + intros. step. constructor.
-    - apply bind_choiceI_bound; auto.
-      + step. constructor. intros. step. constructor.
-      + intros. step. constructor.
-    - apply bind_choiceI_bound; auto.
-      + step. constructor. intros. step. constructor.
-      + intros. step. constructor.
-  Qed.
-
+  (*
   (* TODO: clean up proof *)
-  Lemma interp_state_bounded t c :
+  Lemma interp_state_bounded t :
     choiceI_bound 1 t ->
-    choiceI_bound 1 (interp_state t c).
+    choiceI_bound 1 (interp_state t).
   Proof.
-    unfold interp_state. unfold Interp.interp. unfold iter. unfold MonadIter_stateT0.
-    intros. unfold choiceI_bound. revert t c H. coinduction r CIH.
-    intros. cbn. unfold iter, MonadIter_ctree. rewrite unfold_iter.
+    unfold interp_state. unfold Interp.interp. unfold iter. unfold MonadIter_ctree.
+    intros. unfold choiceI_bound. revert t H. coinduction r CIH.
+    intros. cbn. rewrite unfold_iter.
     cbn. destruct (observe t) eqn:?; cbn. 3: destruct vis.
-    - do 2 rewrite bind_ret_l. cbn. constructor.
+    - rewrite bind_ret_l. constructor.
     - unfold CTree.map. destruct e; destruct s; cbn.
-      + rewrite bind_trigger. do 3 rewrite bind_vis. constructor. intros.
-        do 3 rewrite bind_ret_l. step. constructor; auto.
-        intros. apply CIH. step in H. cbn in H. unfold choiceI_bound_ in H. rewrite Heqc0 in H.
+      + rewrite bind_trigger. rewrite bind_vis. constructor. intros.
+        rewrite bind_ret_l. step. constructor; auto.
+        intros. apply CIH. step in H. cbn in H. unfold choiceI_bound_ in H. rewrite Heqc in H.
         inversion H. invert. apply H1.
-      + rewrite bind_trigger. do 3 rewrite bind_vis. constructor. intros.
-        do 3 rewrite bind_ret_l. step. constructor; auto.
-        intros. apply CIH. step in H. cbn in H. unfold choiceI_bound_ in H. rewrite Heqc0 in H.
+      + rewrite bind_trigger. do 2 rewrite bind_vis. constructor. intros.
+        rewrite bind_trigger. do 2 rewrite bind_vis. step. econstructor. intros.
+        do 2 rewrite bind_ret_l. step. constructor; auto.
+        intros. apply CIH. step in H. cbn in H. unfold choiceI_bound_ in H. rewrite Heqc in H.
         inversion H. invert. apply H1.
-      + rewrite bind_trigger. do 3 rewrite bind_vis. constructor. intros.
-        do 3 rewrite bind_ret_l. step. constructor; auto.
-        intros. apply CIH. step in H. cbn in H. unfold choiceI_bound_ in H. rewrite Heqc0 in H.
+      + rewrite bind_trigger. do 2 rewrite bind_vis. constructor. intros.
+        rewrite bind_trigger. do 2 rewrite bind_vis. step. econstructor. intros.
+        do 2 rewrite bind_ret_l. step. constructor; auto.
+        intros. apply CIH. step in H. cbn in H. unfold choiceI_bound_ in H. rewrite Heqc in H.
         inversion H. invert. apply H1.
     - unfold choice. unfold MonadChoice_ctree. unfold CTree.choice.
-      do 4 rewrite bind_choice. constructor. intros.
-      do 4 rewrite bind_ret_l. step. constructor; auto. intros. apply CIH.
-      step in H. cbn in H. unfold choiceI_bound_ in H. rewrite Heqc0 in H.
+      do 2 rewrite bind_choice. constructor. intros.
+      do 2 rewrite bind_ret_l. step. constructor; auto. intros. apply CIH.
+      step in H. cbn in H. unfold choiceI_bound_ in H. rewrite Heqc in H.
       inversion H. invert. apply H1.
     - unfold choice. unfold MonadChoice_ctree. unfold CTree.choice.
-      do 4 rewrite bind_choice. constructor.
+      do 2 rewrite bind_choice. constructor.
       2: {
-        step in H. cbn in H. unfold choiceI_bound_ in H. rewrite Heqc0 in H.
+        step in H. cbn in H. unfold choiceI_bound_ in H. rewrite Heqc in H.
         inversion H. invert. apply H3.
       }
       intros.
-      do 4 rewrite bind_ret_l. step. constructor; auto. intros. apply CIH.
-      step in H. cbn in H. unfold choiceI_bound_ in H. rewrite Heqc0 in H.
+      do 2 rewrite bind_ret_l. step. constructor; auto. intros. apply CIH.
+      step in H. cbn in H. unfold choiceI_bound_ in H. rewrite Heqc in H.
       inversion H. invert. apply H2.
+  Qed.
+   *)
+  Lemma schedule_spawns t1 t2 :
+    (schedule 1 (fun _ : fin 1 => denote_imp' (Spawn t1 (Spawn t2 Skip))) (Some Fin.F1))
+      ≅
+     TauV (TauV (TauI
+     (schedule 2
+               (cons_vec
+                  (denote_imp' t2)
+                  (fun _ => denote_imp' t1))
+               None))).
+  Proof.
+    rewrite rewrite_schedule. simp schedule_match.
+    cbn. CTree.fold_subst.
+    step. constructor. intros _.
+
+    rewrite rewrite_schedule. simp schedule_match. simp cons_vec.
+    unfold replace_vec. cbn.
+    step. constructor. intros _.
+
+    rewrite rewrite_schedule. simp schedule_match. simp cons_vec. cbn.
+    step. constructor. intros _.
+
+    apply equ_schedule. intro i.
+    dependent destruction i.
+    - simp remove_vec. simp cons_vec. CTree.fold_subst.
+      rewrite bind_ret_l. reflexivity.
+    - dependent destruction i; [| inv i].
+      simp remove_vec. simp cons_vec.
+      unfold remove_front_vec. simp cons_vec. cbn. simp cons_vec.
+      rewrite bind_ret_l. reflexivity.
+      (* rewrite bind_bind. *)
+      (* eapply equ_clo_bind; auto. intros; subst. *)
+      (* rewrite bind_choice. step. constructor. intros. inv i. *)
+  Qed.
+
+  Equations p : fin 2 -> fin 2 :=
+    p Fin.F1 := Fin.FS Fin.F1;
+    p (Fin.FS Fin.F1) := Fin.F1.
+
+  Lemma p_inverse : forall i, p (p i) = i.
+  Proof.
+    intros. dependent destruction i.
+    - simp p; auto.
+    - dependent destruction i. simp p; auto. inv i.
+  Qed.
+
+  Lemma schedule_order (t1 t2 : ctree (parE value) unit)
+    (Hbound1 : choiceI_bound 1 t1)
+    (Hbound2 : choiceI_bound 1 t2) :
+    ChoiceV 2 (fun i' : fin 2 =>
+                 schedule 2
+                          (cons_vec t1 (fun _ => t2))
+                          (Some i')) ~
+    ChoiceV 2 (fun i' : fin 2 =>
+                 schedule 2
+                          (cons_vec t2 (fun _ => t1))
+                          (Some i')).
+  Proof.
+    apply sb_choiceV; intros i; exists (p i); [| symmetry];
+      apply (@schedule_permutation value) with (q:=p);
+      try solve [intros i0; dependent destruction i0; simp cons_vec];
+      try solve [apply p_inverse];
+      try solve [ intros i0; dependent destruction i0;
+                  [| dependent destruction i0; [| inv i0]]; simp p; simp cons_vec; auto].
+  Qed.
+
+  Lemma commut_spawns t1 t2 :
+    schedule_denot' (Spawn t1 (Spawn t2 Skip)) ~
+    schedule_denot' (Spawn t2 (Spawn t1 Skip)).
+  Proof.
+    unfold schedule_denot'.
+    do 2 rewrite schedule_spawns.
+    apply sb_tauV. apply sb_tauV. apply sb_tauI_lr.
+
+    do 2 rewrite rewrite_schedule. simp schedule_match.
+    apply schedule_order; apply denote_stmt_bounded.
+  Qed.
+
+  (* we need 2 yields here since spawning also emits a tau *)
+  (* [| spawn s skip |] = tau tau s
+     (tau at spawn, tau when main thread ends, continue with s) *)
+  (* [| yield; yield; s |] = tau tau s *)
+  Lemma yield_spawn s :
+    schedule_denot' (Seq YieldS (Seq YieldS s)) ~
+    schedule_denot' (Spawn s Skip).
+  Proof.
+    unfold schedule_denot'.
+
+    cbn.
+    do 2 rewrite rewrite_schedule. simp schedule_match.
+    cbn. CTree.fold_subst. do 2 rewrite replace_vec_unary.
+
+    symmetry. apply sb_tauI_r. symmetry.
+
+    rewrite rewrite_schedule. simp schedule_match.
+    apply sb_choiceV_id. intros. dependent destruction x. 2: inv x.
+
+    symmetry.
+    rewrite rewrite_schedule. simp schedule_match.
+    simp cons_vec. cbn.
+    symmetry. apply sb_tauI_r. symmetry.
+    rewrite remove_vec_cons_2.
+
+    do 2 rewrite rewrite_schedule. simp schedule_match.
+    cbn. CTree.fold_subst. apply sb_tauI_r.
+
+    rewrite rewrite_schedule. simp schedule_match.
+    apply sb_choiceV_id. intros. dependent destruction x. 2: inv x.
+    rewrite replace_vec_unary.
+
+    eapply sbisim_schedule.
+    - intro. rewrite bind_ret_l. apply denote_stmt_bounded.
+    - intro. rewrite bind_ret_l. apply denote_stmt_bounded.
+    - intros. do 2 rewrite bind_ret_l. reflexivity.
+  Qed.
+
+  Lemma spawn_skip_equ s :
+    schedule_denot' (Spawn s Skip) ≅ TauV (TauI (TauV (schedule_denot' s))).
+  Proof.
+    unfold schedule_denot'. cbn.
+
+    rewrite rewrite_schedule. simp schedule_match.
+    cbn. CTree.fold_subst.
+    rewrite replace_vec_unary.
+    step. constructor. intros _.
+
+    rewrite rewrite_schedule. simp schedule_match.
+    simp cons_vec. cbn. rewrite remove_vec_cons_2.
+    step. constructor. intros _.
+
+    rewrite rewrite_schedule. simp schedule_match.
+    step. constructor. intros.
+
+    dependent destruction i. 2: inv i.
+    apply equ_schedule. repeat intro. rewrite bind_ret_l. reflexivity.
+  Qed.
+
+  Lemma yield_equ s :
+    schedule_denot' (Seq YieldS s) ≅ TauI (TauV (schedule_denot' s)).
+  Proof.
+    unfold schedule_denot'. cbn.
+
+    rewrite rewrite_schedule. simp schedule_match.
+    cbn. CTree.fold_subst.
+    rewrite replace_vec_unary.
+    step. constructor. intros _.
+
+    rewrite rewrite_schedule. simp schedule_match.
+    step. constructor. intros.
+
+    dependent destruction i. 2: inv i.
+    apply equ_schedule. repeat intro. rewrite bind_ret_l. reflexivity.
+  Qed.
+
+  Lemma spawn_skip_yield s :
+    schedule_denot' (Spawn s Skip) ≈
+    schedule_denot' (Seq YieldS s).
+  Proof.
+    rewrite spawn_skip_equ, yield_equ.
+    rewrite tauI_wb. rewrite tauV_wb.
+    rewrite tauI_wb. rewrite tauV_wb.
+    reflexivity.
+  Qed.
+
+  Lemma spawn_skip s :
+    schedule_denot' (Spawn s Skip) ≈
+    schedule_denot' s.
+  Proof.
+    rewrite spawn_skip_equ.
+    rewrite tauV_wb.
+    rewrite tauI_wb.
+    rewrite tauV_wb.
+    reflexivity.
   Qed.
 
 End Denote1.
